mldsa/src/native/x86_64/src/arith_native_x86_64.h
@@ -103,10 +103,10 @@ void mld_poly_caddq_avx2(int32_t *r);
 
 #if !defined(MLD_CONFIG_NO_VERIFY_API)
 #define mld_poly_use_hint_32_avx2 MLD_NAMESPACE(mld_poly_use_hint_32_avx2)
-void mld_poly_use_hint_32_avx2(int32_t *b, const int32_t *a, const int32_t *h);
+void mld_poly_use_hint_32_avx2(int32_t *a, const int32_t *h);
 
 #define mld_poly_use_hint_88_avx2 MLD_NAMESPACE(mld_poly_use_hint_88_avx2)
-void mld_poly_use_hint_88_avx2(int32_t *b, const int32_t *a, const int32_t *h);
+void mld_poly_use_hint_88_avx2(int32_t *a, const int32_t *h);
 #endif /* !MLD_CONFIG_NO_VERIFY_API */
 
 #define mld_poly_chknorm_avx2 MLD_NAMESPACE(mld_poly_chknorm_avx2)
