proofs/cbmc/poly_use_hint_c/poly_use_hint_c_harness.c
@@ -5,11 +5,11 @@
 
 // Prototype for the function under test
 #define mld_poly_use_hint_c MLD_ADD_PARAM_SET(mld_poly_use_hint_c)
-void mld_poly_use_hint_c(mld_poly *b, mld_poly *a, mld_poly *h);
+void mld_poly_use_hint_c(mld_poly *a, mld_poly *h);
 
 
 void harness(void)
 {
-  mld_poly *a, *b, *h;
-  mld_poly_use_hint_c(b, a, h);
+  mld_poly *a, *h;
+  mld_poly_use_hint_c(a, h);
 }
