proofs/cbmc/poly_use_hint_native_aarch64/poly_use_hint_native_aarch64_harness.c
@@ -6,19 +6,19 @@
 #include "params.h"
 
 #if MLDSA_GAMMA2 == ((MLDSA_Q - 1) / 88)
-int mld_poly_use_hint_88_native(int32_t *b, const int32_t *a, const int32_t *h);
+int mld_poly_use_hint_88_native(int32_t *a, const int32_t *h);
 #else
-int mld_poly_use_hint_32_native(int32_t *b, const int32_t *a, const int32_t *h);
+int mld_poly_use_hint_32_native(int32_t *a, const int32_t *h);
 #endif
 
 void harness(void)
 {
-  int32_t *b, *a, *h;
+  int32_t *a, *h;
   int t;
 
 #if MLDSA_GAMMA2 == ((MLDSA_Q - 1) / 88)
-  t = mld_poly_use_hint_88_native(b, a, h);
+  t = mld_poly_use_hint_88_native(a, h);
 #else
-  t = mld_poly_use_hint_32_native(b, a, h);
+  t = mld_poly_use_hint_32_native(a, h);
 #endif
 }
